stdlib/ptr/output/ptr/proofs/proof_const_ptr_add.v
@@ -22,11 +22,10 @@ Proof.
       - if T is a ZST, then the wrapped offset gets annihilated everywhere, so it's fine.
       - else, we also know that it's in isize_t, so it's same as before.
     *)
-  4,6: rewrite /OffsetLocSt; simplify_layout (use_layout_alg' (ty_syn_type T_ty)); do 2 f_equiv.
+  4,6: rewrite /OffsetLocSt; simplify_layout (use_layout_alg' (ty_syn_type T_ty)); f_equiv.
   all: destruct (decide (ly_size T_st_ly = 0%nat));
     [ lia | assert (MinInt isize_t ≤ count ≤ MaxInt isize_t)%Z by solve_goal with nia; sidecond_hammer].
-  all: rewrite wrap_to_int_id'.
-  all: sidecond_hammer.
+  all: rewrite wrap_to_int_id'; sidecond_hammer.
 
   Unshelve. all: print_remaining_sidecond.
 Qed.
