theories/rust_typing/ltype_rules.v
@@ -170,10 +170,10 @@ Proof.
   destruct b1, b2; try done; unfold bor_kind_direct_incl.
   + iDestruct "Hincl" as "->"; eauto.
   + rewrite !ltype_own_enum_unfold /enum_ltype_own.
-    iIntros "(%el & %Hen & %Hly & Hlb & ? & [])".
+    iIntros "(%el & %Hen & %Hly & Hlb & [])".
   + rewrite !ltype_own_enum_unfold /enum_ltype_own.
     iDestruct "Hincl" as "(Hincl & ->)".
-    iIntros "(%el & %Hen & %Hly & Hlb & ? & [])".
+    iIntros "(%el & %Hen & %Hly & Hlb & [])".
 Qed.
 
 
@@ -1023,9 +1023,9 @@ Section guarded.
     (∀ m, m < n → P ≡{m}≡ Q) →
     guarded P ≡{n}≡ guarded Q.
   Proof.
-    rewrite /guarded. 
+    rewrite /guarded.
     intros Hle. f_contractive.
-    by apply Hle. 
+    by apply Hle.
   Qed.
 End guarded.
 
